implemented is_even proof

test/lean/Proofs.lean
@@ -82,7 +82,7 @@ lemma BigInt.update_eq (l : List U64) (i : Int) (x : U64)
   rw [List.len_eq_length]
   apply h
 
-def BigInt.val {N : Usize} (x : biginteger.BigInt N) : Int := valImpl (Array.v x)
+def BigInt.val {N : Usize} (x : biginteger.BigInt N) : Int := valImpl x.v
 
 def BigInt.mod_value (n : Int) : Int := (U64.max + 1) ^ (Int.toNat n)
 
@@ -417,6 +417,37 @@ lemma add_with_carry_correct :
     unfold BigInt.val
     unfold BigInt.mod_value
     simp [*]
+
+lemma is_even_correct :
+  ∀ (N : Usize) (self: BigInt N) (h: 0 < N.val),
+  ∃ b, biginteger.BigInt.const_is_even N self = .ok b ∧ b = (self.val % 2 = 0) := by {
+    intro N self h
+    unfold biginteger.BigInt.const_is_even
+    progress with Array.index_usize_spec as ⟨ idef, idecl ⟩ 
+    progress as ⟨ is_even_def, is_even_decl ⟩
+    simp
+    rw [Scalar.eq_equiv]
+    rw [is_even_decl]
+    rw [idecl]
+    simp [*]
+    unfold BigInt.val
+    unfold valImpl
+    match h_self : self.v with
+    | x::xs => {
+      unfold List.index
+      simp only [h_self]
+      simp only [↓reduceIte]
+      rw [Int.add_emod]
+      rw [Int.mul_emod]
+      simp
+    }
+    | [] => {
+      have h_contr := BigInt.len_spec N self
+      simp [h_self] at h_contr
+      rw [←h_contr] at h
+      simp at h
+    }
+  }
 
 -- end arithmetics
 
